Refinery/Term/Extrinsic/Wk.lean
@@ -1,0 +1,8 @@
+import Refinery.Term.Syntax
+import Refinery.Ctx.Basic
+
+namespace Refinery
+
+namespace Term
+
+variable {α : Type v} {ε : Type w} [HasQuant α] [PartialOrder ε]
